Solved goals return a subst + state

code/rocq/det.v
@@ -74,14 +74,14 @@ Inductive expand_res :=
   | Expanded of state
   | CutBrothers of state
   | Failure
-  | Solved of Sigma.
+  | Solved of Sigma & state.
 
-Definition mkAnd left r :=
+Definition mkAnd alt left r :=
   match r with
   | Failure => Failure
   | Expanded st => Expanded (And left st)
   | CutBrothers st => CutBrothers (And left st)
-  | Solved s => Solved s
+  | Solved s A => Solved s (And alt A)
   end.
 
 Definition mkOr left sr r :=
@@ -89,7 +89,7 @@ Definition mkOr left sr r :=
   | Failure => Failure
   | Expanded st => Expanded (Or left sr st)
   | CutBrothers st => Expanded (Or left sr st) (* for now this is the rightmost brother *)
-  | Solved s => Solved s
+  | Solved s A => Solved s A
   end.
 
 Fixpoint cut st :=
@@ -126,7 +126,7 @@ Fixpoint big_or pr (s : seq (Sigma * R)) : state :=
 Fixpoint expand s (st :state) : expand_res :=
   match st with
   | KO => Failure
-  | OK => Solved s
+  | OK => Solved s KO
   | CutOut => Failure
   | Goal _ Cut  => CutBrothers OK
   | Goal pr (App (v _) _) => Failure
@@ -136,14 +136,14 @@ Fixpoint expand s (st :state) : expand_res :=
       else Expanded KO
   | Or st1 sr st2 =>
       match expand s st1 with
-      | Solved s => Solved s
+      | Solved s A => Solved s (Or A sr st2)
       | Expanded st1 => Expanded (Or st1 sr st2)
       | CutBrothers st1 => Expanded (Or st1 sr (cut st2))
       | Failure => mkOr st1 sr (expand sr st2)
       end
   | And st1 st2 =>
       match expand s st1 with
-      | Solved s1 => mkAnd st1 (expand s1 st2)
+      | Solved s1 r => mkAnd r st1 (expand s1 st2)
       | Expanded st1 => Expanded (And st1 st2)
       | CutBrothers st1 => CutBrothers (And st1 st2)
       | Failure => Failure
@@ -151,162 +151,162 @@ Fixpoint expand s (st :state) : expand_res :=
   end
 .
 
-Inductive run_res := Done of Sigma | Failed.
+Inductive run_res := Done of Sigma & state | Failed.
 
-Inductive run : Sigma -> state -> run_res -> state -> Prop :=
-  | run_done {s s' A} : expand s A = Solved s' -> run s A (Done s') A
-  | run_fail {s A B}  : expand s A = Failure   -> run s A Failed B
-  | run_cut {s s' A B C} : expand s A = CutBrothers B -> run s B s' C -> run s A s' C
-  | run_step {s s' A B C} : expand s A = Expanded B  -> run s B s' C -> run s A s' C.
+Inductive run : Sigma -> state -> run_res -> Prop :=
+  | run_done {s s' A alt} : expand s A = Solved s' alt  -> run s A (Done s' alt)
+  | run_fail {s A}  : expand s A = Failure   -> run s A Failed
+  | run_cut {s s' A B} : expand s A = CutBrothers B -> run s B s' -> run s A s'
+  | run_step {s s' A B} : expand s A = Expanded B  -> run s B s' -> run s A s'.
 
-Inductive expand_no_cut_failure : Sigma -> state -> state -> Prop :=
+Inductive expand_no_cut_failure : Sigma -> state -> Prop :=
   | expand_no_cut_failure_fail {s A} :
-      expand s A = Failure -> expand_no_cut_failure s A A
-  | expand_no_cut_failure_step {s A B C} :
-      expand s A = Expanded B  -> expand_no_cut_failure s B C -> expand_no_cut_failure s A C.
+      expand s A = Failure -> expand_no_cut_failure s A
+  | expand_no_cut_failure_step {s A B} :
+      expand s A = Expanded B  -> expand_no_cut_failure s B -> expand_no_cut_failure s A.
 
 Inductive expand_no_cut : Sigma -> state -> Prop :=
-  | expand_no_cut_solved {s' s A} : expand s A = Solved s' -> expand_no_cut s A
+  | expand_no_cut_solved {s' s A alt} : expand s A = Solved s' alt -> expand_no_cut s A
   | expand_no_cut_failure1 {s A}  : expand s A = Failure   -> expand_no_cut s A
   | expand_no_cut_expanded {s A B}: expand s A = Expanded B -> expand_no_cut s B -> expand_no_cut s A.
 
-Lemma run_Solved_id {s s1 A B r}:
-    expand s A = Solved s1 -> run s A r B -> r = Done s1 /\ A = B.
+Lemma run_Solved_id {s s1 A r alt}:
+    expand s A = Solved s1 alt -> run s A r -> r = Done s1 alt.
 Proof.
-  move=> + H.
-  by case: H => //=; clear; [move=> s A s3 H1; rewrite H1=> -[] ?; subst => //= | | | ]; congruence.
+  move=> + H; by case: H => //=; clear; congruence.
 Qed.
 
-Lemma run_Failure_and_Done {s s' A A'}:
-  expand s A = Failure -> run s A (Done s') A' -> False.
+Lemma run_Failure_and_Done {s s' A alt}:
+  expand s A = Failure -> run s A (Done s' alt) -> False.
 Proof. by inversion 2; subst; congruence. Qed.
 
-Lemma done_fail {s}: Done s <> Failed. by []. Qed.
-
-Lemma run_consistent: forall {s0 A s1 s2 B C},
-  run s0 A s1 B -> run s0 A s2 C -> s1 = s2 /\ (s1 <> Failed -> B = C).
+Lemma run_consistent: forall {s0 A s1 s2},
+  run s0 A s1 -> run s0 A s2 -> s1 = s2.
 Proof.
-  move=> s0 A s1 + B  + H.
+  move=> s0 A s1 + H.
   elim:H; clear.
-  + move=> s s' A H B C H1.
-    by move: (run_Solved_id H H1) => []??; subst.
-  + move=> s st st1 H B C H0.
-    inversion H0; subst; clear H0 => //=; by rewrite H in H1.
-  + move=> s st st1 st2 r H H1 IH B C H2.
-    inversion H2; subst => //; rewrite H in H0; try by [].
-    by move: H0 => -[] ?; subst; auto.
-  + move=> s st st1 st2 r H H1 IH B C H2.
-    inversion H2; subst; clear H2; rewrite H in H0; try by [].
-    by move: H0 => [] ?; subst; auto.
+  + move=> s s' A alt H B H1.
+    by move: (run_Solved_id H H1).
+  + move=> s st st1 H H0.
+    by inversion H0; congruence.
+  + move=> s st st1 st2 + H1 IH H H2.
+    inversion H2; subst; try congruence => //; rewrite H0 => -[]?; subst; by auto.
+  + move=> s st st1 st2 + H1 IH B H2.
+    inversion H2; subst; clear H2; try congruence; rewrite H0 => -[]?; subst; by auto.
 Qed.
 
-Lemma run_cut_simpl {pr s2 s3 B}:
-  run s3 (Goal pr Cut) (Done s2) B -> expand s3 OK = Solved s2 /\ B = OK.
+Lemma run_cut_simpl {pr s2 s3 alt}:
+  run s3 (Goal pr Cut) (Done s2 alt) -> expand s3 OK = Solved s2 alt.
 Proof. by inversion 1; move: H1 => //= [] ?; subst; inversion H2; subst. Qed.
 
-Lemma run_and_complete {s s' A B C} :
-  run s (And A B) (Done s') C ->
-    (exists il ir s'', C = And il ir /\ run s A (Done s'') il /\ run s'' B (Done s') ir).
+Lemma run_and_complete {s s' altAB A B} :
+  run s (And A B) (Done s' altAB) ->
+    (exists s'' altA altB, altAB = And altA altB /\ run s A (Done s'' altA) /\ run s'' B (Done s' altB)).
 Proof.
   remember (And _ _) as g0 eqn:Hg0.
-  remember (Done _) as s1 eqn:Hs1 => H.
-  elim: H A B Hg0 s' Hs1; clear => //=.
-  - move=> s s' AB + A B ? s'' [] ?; subst => //=.
-    case L: expand => [|||x] //; case R: expand => //= -[?]; subst.
-    by exists A, B, x; repeat constructor.
-  - move=> s s' ? B C + H1 + A B' ? s'' ?; subst => //=.
+  remember (Done _ _) as s1 eqn:Hs1 => H.
+  elim: H A B altAB Hg0 s' Hs1; clear => //=.
+  - move=> s s' AB alt + A B alt' ? s'' [] ??; subst => //=.
+    case L: expand => [|||x] //; case R: expand => //= -[]??; subst.
+    do 3 eexists; repeat constructor.
+    + apply L.
+    + apply R. 
+  - move=> s s' ? B + H1 + A B' alt ? s'' ?; subst => //=.
     case L: expand => [|AC||s'] // => [[?]|]; subst.
-    - move=> /(_ _ _ erefl _ erefl) [il [ir [s']]] [-> [ IHl IHr]].
-      exists il, ir, s'; split=> //; split.
+    - move=> /(_ _ _ _ erefl _ erefl) [s'[altA[altB[?[IHl IHr]]]]]; subst.
+      do 3 eexists; repeat split => //=.
       by apply: run_cut L IHl.
       by apply: IHr.
     - case R: expand => //= -[?]; subst.
-      move=> /(_ _ _ erefl _ erefl) [il [ir [s''']]] [-> [ IHl IHr]].
-      exists il, ir, s'''; split=> //; split.
+      move=> /(_ _ _ _ erefl _ erefl) [s''' [altA [altB [? [IHl IHr]]]]]; subst.
+      move: (run_Solved_id L IHl) => [] ?; subst.
+      do 3 eexists; repeat split => //=.
       - by apply: IHl.
-      - move: (run_Solved_id L IHl) => [] []??; subst.
-        apply: run_cut R IHr.
-  - move=> s ? A' C ? + H1 + A B ? s' ?; subst => //=.
+      - apply: run_cut R IHr.
+  - move=> s ? A' C + H1 + A B ? s' ??; subst => //=.
     case E1: expand => //= [|s1].
-    - move=> [?]; subst.
-      move => /(_ _ _ erefl _ erefl) [il [ir [s''']]] [-> [ IHl IHr]].
-      exists il, ir, s'''; repeat split => //=.
+    - move=> []?; subst.
+      move => /(_ _ _ _ erefl _ erefl) [s''' [altA [altB [? [IHl IHr]]]]]; subst.
+      do 3 eexists; repeat split => //=.
       by apply: run_step E1 IHl.
+      by assumption.
     - case E2: expand => //= [st] [] ?; subst.
-      move=> /(_ _ _ erefl _ erefl) [il [ir [s''']]] [? [ IHl IHr]]; subst.
-      move: (run_Solved_id E1 IHl) => [][] ??; subst.
-      exists il, ir, s1; repeat split => //=.
+      move=> /(_ _ _ _ erefl _ erefl) [s''' [altA [altB [?[IHl IHr]]]]]; subst.
+      move: (run_Solved_id E1 IHl) => []??; subst.
+      do 3 eexists; repeat split => //=.
+      eassumption.
       apply: run_step E2 IHr.
 Qed.
 
-Lemma run_and_correct {s0 s1 s2 A B A' B'} :
-    run s0 A (Done s1) A' -> run s1 B (Done s2) B' ->
-      run s0 (And A B) (Done s2) (And A' B').
+Lemma run_and_correct {s0 s1 s2 A B altA altB} :
+    run s0 A (Done s1 altA) -> run s1 B (Done s2 altB) ->
+      run s0 (And A B) (Done s2 (And altA altB)).
 Proof.
-  remember (Done _) as D eqn:HD => H.
-  elim: H s1 s2 B B' HD => //=; clear.
-  + move=> + s1 + + s1' s2 B B' [] ? H1; subst.
-    remember (Done s2) as D eqn:HD.
-    elim: H1 s2 HD => //=; clear.
-    + move=> s s' A H s2 [] ? s0 A' H1; subst.
+  remember (Done _ _) as D eqn:HD => H.
+  elim: H altA s1 s2 B altB HD => //=; clear.
+  + move=> + + + + + + s1' s2 B altB + H1.
+    remember (Done s2 _) as D eqn:HD.
+    elim: H1 s2 altB HD => //=; clear.
+    + move=> s s' A altA H altB s2 [] ?? s0 s1 A' altA' H1 altA'' []??; subst.
       apply: run_done => //=; rewrite H1 H => //=.
-    + move=> s s' A B C H H1 IH s2 ? s0 A' H2; subst.
+    + move=> s s' A B H H1 IH s2 altB ? s0 s1 A' altA' H2 altA []??; subst.
       apply: run_cut => //=.
       + rewrite H2 H => //=.
       + apply: IH => //=.
-    + move=> s ? A B C H H1 IH s' ? s'' A' H2; subst.
+      + eassumption.
+    + move=> s ? A B H H1 IH s' ? s'' A' H2 A0 altA0 H3 altA'' [] ??; subst.
       apply: run_step => //=.
-      + by rewrite H2 H.
-      + by apply: IH _ H2.
-  + move=> s s' A CA CA' H H1 IH s1 s2 B B' ? H2; subst.
+      + by rewrite H3 H.
+      + by apply: IH erefl.
+  + move=> s s' A CA H H1 IH altA s1 s2 B altB ? H2; subst.
     apply: run_cut => //=.
     + by rewrite H.
     + by apply: IH _ H2.
-  + move=> s s' A AE AE' H H1 IH s1 s2 B B' ? H2; subst.
+  + move=> s s' A AE H H1 IH altA s1 s2 B altB ? H2; subst.
     apply: run_step => //=.
     + by rewrite H.
     + by apply: IH erefl H2.
 Qed.
 
-Lemma run_and_fail {s A B C}:
-  run s (And A B) Failed C ->
-    run s A Failed C \/ (exists s' C', run s A (Done s') C' /\ run s' B Failed C).
+Lemma run_and_fail {s A B}:
+  run s (And A B) Failed ->
+    run s A Failed \/ (exists s' altA, run s A (Done s' altA) /\ run s' B Failed).
 Proof.
   move=> H.
   remember (And _ _) as R eqn:HR.
   remember Failed as F eqn:HF.
   elim: H A B HR HF => //=; clear.
-  + move=> s A B + A1 B2 ? _; subst => //=.
+  + move=> s A + A1 B2 ? _; subst => //=.
     case E: expand => [|||s'] //=.
     + by move=> _; left; apply: run_fail.
     + case F: expand => //= _; right.
-      exists s', A1; split.
-      - by apply run_done.
+      do 2 eexists; split.
+      - apply: run_done E.
       - by apply run_fail.
-  + move=> s s' A B C + H1 IH A1 B1 ? ?; subst => //=.
+  + move=> s s' A B + H1 IH A1 B1 ? ?; subst => //=.
     case E: expand => //=.
     - move=> [] ?; subst.
       move: (IH _ _ erefl erefl) => [].
       + by left; apply: run_cut E _.
-      + move=> [? [? []]] H2 H3.
-        by right; do 2 eexists; split; [|eassumption]; apply: run_cut E H2.
+      + move=> [] s' [] altA [] H2 H3.
+        right; do 2 eexists; split; [|eassumption]; apply: run_cut E H2.
     - case F: expand => //= -[] ?; subst.
       move: (IH _ _ erefl erefl) => []; [by auto|].
-      move=> [? [? []]] H2 H3.
-      move: (run_Solved_id E H2) => [][]??; subst.
-      right; do 2 eexists; split; [eassumption|apply: run_cut F H3].
-  + move=> s s' A B C + H1 IH A1 B1 ??; subst => //=.
+      move=> [] s' [] altA [] H2 H3.
+      move: (run_Solved_id E H2) => []?; subst.
+      right; repeat eexists; [eassumption|apply: run_cut F H3].
+  + move=> s s' A B + H1 IH A1 B1 ??; subst => //=.
     case E: expand => //=.
     + move=> [] ?; subst.
       move: (IH _ _ erefl erefl) => [] {IH}.
       + by left; apply: run_step E _.
-      + move=> [? [? []]] H2 H3.
-        by right; do 2 eexists; split; [apply: run_step E H2|].
+      + move=> [] ? [] altA [] H2 H3.
+        by right; repeat eexists; [apply: run_step E H2|].
     + case F: expand => //= -[] ?; subst.
       move: (IH _ _ erefl erefl) => [] {IH}; [by auto|].
-      move=> [? [? []]] H2 H3.
-      move: (run_Solved_id E H2) => [][]??; subst.
-      right; do 2 eexists; split; [by eassumption|].
+      move=> [] ? [] altA [] H2 H3.
+      move: (run_Solved_id E H2) => []?; subst.
+      right; repeat eexists; [by eassumption|].
       by apply: run_step F H3.
 Qed.
 
@@ -320,18 +320,18 @@ Proof.
   by move=> s A B H H1 IH B1 +; rewrite H => -[] ?; subst.
 Qed.
 
-Lemma expand_cut_fail {s s' A}:
-  expand s (cut A) = Solved s' -> False.
+Lemma expand_cut_solved {s s' A altA}:
+  expand s (cut A) = Solved s' altA -> False.
 Proof.
-  elim: A s s' => //=.
-  + move=> A H1 s B H2 s1 s2.
+  elim: A s s' altA => //=.
+  + move=> A H1 s B H2 s1 s2 altA.
     case E: expand => //=.
-    + case F: expand => //= -[] ?; subst.
+    + case F: expand => //= -[] ??; subst.
       apply: H2 F.
-    + by move=> [] ?; subst; apply: H1 E.
-  + move=> A IH1 B IH2 s s'.
+    + by move=> [] ??; subst; apply: H1 E.
+  + move=> A IH1 B IH2 s s' altA.
     case E: expand => //=.
-    case F: expand => //= -[] ?; subst.
+    case F: expand => //= -[] ??; subst.
     apply: IH2 F.
 Qed.
 
@@ -346,7 +346,7 @@ Proof.
     case X: expand => //=.
     + move=> [] ?; subst; apply: IHA X.
     + case: expand => //=? -[]?; subst.
-      apply: expand_cut_fail X.
+      apply: expand_cut_solved X.
 Qed.
 
 Lemma expand_cut_expanded {s A B}: expand s (cut A) = Expanded B -> False.
@@ -374,241 +374,222 @@ Proof.
   + by right; eexists.
   + by move: (expand_cut_CB X).
   + by left.
-  + by move: (expand_cut_fail X).
+  + by move: (expand_cut_solved X).
 Qed.
 
-Lemma run_cut_fail {s s' A B} :
-  run s (cut A) (Done s') B -> False.
+Lemma run_cut_fail {s s' A altA} :
+  run s (cut A) (Done s' altA) -> False.
 Proof.
-  remember (cut A) as C eqn:HC.
-  remember (Done s') as D eqn:HD.
-  move=> H.
-  elim: H s' A HC HD; clear => //=.
-  + by move=> ??? H ?? ? [] ?; subst; apply: expand_cut_fail H.
-  + move=> s r A B C H H1 IH A' s' ??; subst.
-    by move: (expand_cut_CB H).
-  + move=> s r A B C H H1 IH A' s' ??; subst.
-    by apply expand_cut_expanded in H.
+  inversion 1; subst.
+  + by move: (expand_cut_solved H4).
+  + by move: (expand_cut_CB H1).
+  + by move: (expand_cut_expanded H1).
 Qed.
 
-Lemma expand_no_cut_failure_split {s A B AB}: 
-  expand_no_cut_failure s (And A B) AB ->
-    (exists A', expand_no_cut_failure s A A') \/ 
-      (exists s' A' B', run s A (Done s') A' /\ expand_no_cut_failure s' B B').
+Lemma expand_no_cut_failure_split {s A B}: 
+  expand_no_cut_failure s (And A B) ->
+    (expand_no_cut_failure s A) \/ 
+      (exists s' altA, run s A (Done s' altA) /\ expand_no_cut_failure s' B).
 Proof.
   remember (And A B) as And eqn:HAnd.
   move=> H; elim: H A B HAnd; clear.
   + move=> s ? + A B ?; subst => //=.
     case X: expand => //=.
-    + by left; eexists A; apply: expand_no_cut_failure_fail.
-    + case Y: expand => //= _; right; do 3 eexists; split.
+    + by left; apply: expand_no_cut_failure_fail.
+    + case Y: expand => //=  _; right; repeat eexists.
       + apply: run_done X.
       + by apply: expand_no_cut_failure_fail.
-  + move=> s st st1 st2 + H1 + A B ?; subst => //=.
+  + move=> s st st1 + H1 + A B ?; subst => //=.
     case X: expand => //=.
     + move=> []?;subst.
-      move=> /(_ _ _ erefl) [] [].
-      + move=> X1 H; left; eexists; apply: expand_no_cut_failure_step X H.
-      + move=> X1 [X2 [H2 [H3 H4]]]; right.
-        do 3 eexists; repeat split.
-        + apply: run_step X H3.
-        + apply: H4.
+      move=> /(_ _ _ erefl) [].
+      + move=> H; left; apply: expand_no_cut_failure_step X H.
+      + move=> [X1 [altA [H2 H3]]]; right.
+        repeat eexists.
+        + apply: run_step X H2.
+        + apply: H3.
     + case Y: expand => //= [A'] [] ?; subst.
       move=> /(_ _ _ erefl) [].
       + by left.
-      + move=> [s' [A'' [B' [H2 H3]]]]; right.
-        do 3 eexists; repeat split; try eassumption.
+      + move=> [s' [altA [H2 H3]]]; right.
+        repeat eexists; try eassumption.
         inversion H2; subst; try congruence; clear H2.
-        move: H6; rewrite X => -[]?; subst.
+        move: H6; rewrite X => -[]??; subst.
         by apply: expand_no_cut_failure_step Y H3.
 Qed.
 
-Lemma run_or_done_cut {s1 s2 SOL A A' B}:
-  run s1 A (Done SOL) A' ->
-  run s1 (Or A s2 (cut B)) (Done SOL) (Or A' s2 (cut B)).
+Lemma run_or_done_cut {s1 s2 SOL A B altA}:
+  run s1 A (Done SOL altA) ->
+  run s1 (Or A s2 (cut B)) (Done SOL (Or altA s2 (cut B))).
 Proof.
-  remember (Done _) as D eqn:HD.
+  remember (Done _ _) as D eqn:HD.
   move=> H.
-  elim: H s2 SOL B HD; clear => //=.
-  + move=> s st s' H s2 SOL B [] ?; subst.
+  elim: H altA s2 SOL B HD; clear => //=.
+  + move=> s st s' alt H altA s2 SOL B [] ??; subst.
     by apply: run_done => //=; rewrite H.
-  + move=> s st st1 st2 r H H1 IH s2 SOL B H2; subst.
+  + move=> s st st1 st2 H H1 IH s2 SOL B H2 ?; subst.
     apply: run_step => //=.
     + by rewrite H.
     + by rewrite cut_cut_same; apply: IH erefl.
-  + move=> s st st1 st2 r H H1 IH s2 SOL B0 ?; subst.
+  + move=> s st st1 st2 H H1 IH s2 SOL B0 ??; subst.
     apply: run_step => //=.
     + by rewrite H.
     + by apply: IH.
 Qed.
 
-Lemma run_or_correct_left {s s' A A'}:
-  run s A (Done s') A' ->
-    forall s2 B, exists B', run s (Or A s2 B) (Done s') (Or A' s2 B').
+Lemma run_or_correct_left {s s' A altA}:
+  run s A (Done s' altA) ->
+    forall s2 B, exists altB, run s (Or A s2 B) (Done s' (Or altA s2 altB)).
 Proof.
-  remember (Done _) as D eqn:HD => H.
-  elim: H s' HD => //=; clear.
-  + move=> s st s' H s'' [] ? s2 B; subst.
-    by exists B; apply: run_done => //=; rewrite H.
-  + move=> s A st1 st2 r H H1 IH s' ? s2 B; subst.
-    exists (cut B).
-    apply: run_step => //=.
+  remember (Done _ _) as D eqn:HD => H.
+  elim: H s' altA HD => //=; clear.
+  + move=> s st s' alt H s'' altA [] ?? s2 B; subst.
+    by eexists; apply: run_done => //=; rewrite H.
+  + move=> s A st1 st2 H H1 IH s' altA ? s2 B; subst.
+    eexists; apply: run_step => //=.
     + by rewrite H.
     + by apply: run_or_done_cut H1.
-  + move=> s st st1 st2 r H H1 IH s' ? s2 B; subst.
-    move: (IH s' erefl s2 B) => [B' H2].
-    exists B'; apply: run_step _ H2 => //=.
+  + move=> s st st1 st2 H H1 IH s' altA ? s2 B; subst.
+    move: (IH s' altA erefl s2 B) => [altB H2].
+    eexists; apply: run_step _ H2 => //=.
     by rewrite H.
 Qed. 
 
-Lemma run_or_correct_right {s1 s2 s3 A A' B B'}:
-  expand_no_cut_failure s1 A A' -> run s2 B (Done s3) B' ->
-    (exists B', run s1 (Or A s2 B) (Done s3) (Or A' s2 B')).
+Lemma run_or_correct_right {s1 s2 s3 A B altB}:
+  expand_no_cut_failure s1 A -> run s2 B (Done s3 altB) ->
+    (run s1 (Or A s2 B) (Done s3 altB)).
 Proof.
   move=> H.
-  elim: H s2 B B' s3; clear.
-  + move=> + + + s2 B B' s3 H1.
-    remember (Done s3) as DS eqn:HDS.
-    elim: H1 s3 HDS => //=; clear.
-    + move=> s2 B s3 H s3' [] ? s1 A H1; subst.
-      by eexists; apply: run_done =>//=; rewrite H1 H.
-    + move=> s2 B BC B' r H H1 + s3 ? s1 A H2; subst.
-      move=> /(_ _ erefl _ _ H2) [B2 IH]; eexists.
+  elim: H s2 B altB s3; clear.
+  + move=> + + + s2 B altB s3 H1.
+    remember (Done s3 _) as DS eqn:HDS.
+    elim: H1 altB s3 HDS => //=; clear.
+    + move=> s2 s3 B altB H s3' s4 [] ?? s1 A H1; subst.
+      by apply: run_done =>//=; rewrite H1 H.
+    + move=> s2 s' B BC H H1 + s3 A ? s1 A' H2; subst.
+      move=> /(_ _ _ erefl _ _ H2) IH.
       apply: run_step _ IH => //=.
       by rewrite H2 H.
-    + move=> s2 B BE B' r H H1 + s3 ? s1 A H2; subst.
-      move=> /(_ _ erefl _ _ H2) [B2 IH]; eexists.
+    + move=> s2 s' B BE H H1 + altB s3 ? s1 A H2; subst.
+      move=> /(_ _ _ erefl _ _ H2) IH.
       apply: run_step _ IH => //=.
       by rewrite H2 H.
-  + move=> s1 A EA A' H H1 + s2 B B' s3 H2.
-    move=> /(_ _ _ _ _ H2) [B2 IH]; eexists.
+  + move=> s1 A EA H H1 + s2 B altB B' H2.
+    move=> /(_ _ _ _ _ H2) => IH.
     apply: run_step _ IH => //=.
     by rewrite H.
 Qed.
 
-Lemma run_or_correct {s1 s2 A B SOL A' B'}:
-  (run s1 A (Done SOL) A') \/ 
-    (expand_no_cut_failure s1 A A' /\ run s2 B (Done SOL) B') ->
-      exists B', run s1 (Or A s2 B) (Done SOL) (Or A' s2 B').
+Lemma run_or_correct {s1 s2 A B SOL altA altB}:
+  (run s1 A (Done SOL altA)) \/ 
+    (expand_no_cut_failure s1 A /\ run s2 B (Done SOL altB)) ->
+      exists altAB, run s1 (Or A s2 B) (Done SOL altAB).
 Proof.
   move=> [].
-  + move=> H; apply: run_or_correct_left H _ _.
-  + move=> []; apply: run_or_correct_right.
-Qed.
-
-Lemma run_or_done {s1 s2 A B SOL r}:
-  run s1 (Or A s2 B) (Done SOL) r -> exists x y, r = Or x s2 y.
-Proof.
-  remember (Or _ _ _) as O eqn:HO.
-  remember (Done _) as D eqn:HD.
-  move=> H.
-  elim: H s2 A B SOL HO HD; clear => //=.
-  + by move=> s st s' H s2 A B SOL ? [] ?; subst; do 2 eexists.
-  + move=> s st st1 st2 r + H1 IH s2 A B SOL ??; subst => //=.
-    by case E: expand => //=; case E: expand => //=.
-  + move=> s st st1 st2 r + H1 IH s2 A B SOL ??; subst => //=.
-    case E: expand => //= [A'|A'|].
-    + by move=> [] ?; subst; move: (IH s2 A' B SOL erefl erefl).
-    + by move=> [] ?; subst; move: (IH s2 A' (cut B) SOL erefl erefl).
-    + case F: expand => //= -[]?; subst; by move: (IH _ _ _ SOL erefl erefl).
+  + move=> H; move: (run_or_correct_left H s2 B) => [altB1 H1]; eexists; apply H1.
+  + by move=> [] H1 H2; move: (run_or_correct_right H1 H2); exists altB.
 Qed.
 
 Lemma run_and_done {s A B SOL r}:
-  run s (And A B) (Done SOL) r -> exists x y, r = And x y.
+  run s (And A B) (Done SOL r) -> exists x y, r = And x y.
 Proof.
   remember (And _ _) as O eqn:HO.
-  remember (Done _) as D eqn:HD.
+  remember (Done _ _) as D eqn:HD.
   move=> H.
   elim: H A B SOL HO HD; clear => //=.
-  + by move=> s st s' H A B SOL ? [] ?; subst; do 2 eexists.
-  + move=> s st st1 st2 r + H1 IH A B SOL ??; subst => //=.
+  + move=> s s' A altA + A' B H SOL [] ??; subst => //=.
+    case X: expand => //=.
+    case Y: expand => //= -[] ??; subst.
+    by do 2 eexists.
+  + move=> s st st1 st2 + H1 IH A B SOL ??; subst => //=.
     case E: expand => //=.
     + by move=> []?; subst; apply: IH erefl erefl.
     + by case F: expand => //= -[]?; subst; apply: IH erefl erefl.
-  + move=> s st st1 st2 r + H1 IH A B SOL ??; subst => //=.
+  + move=> s st st1 st2 + H1 IH A B SOL ??; subst => //=.
     case E: expand => //= [A'|A'].
     + by move=> [] ?; subst; apply: IH erefl erefl.
     + by case F: expand => //= -[]?; subst; apply: IH erefl erefl.
 Qed.
 
-Lemma run_or_complete {s1 s2 A B SOL A' B'}:
-  run s1 (Or A s2 B) (Done SOL) (Or A' s2 B') ->
-    run s1 A (Done SOL) A' \/ 
-      expand_no_cut_failure s1 A A' /\ run s2 B (Done SOL) B'.
+Lemma run_or_complete {s1 s2 A B SOL altAB}:
+  run s1 (Or A s2 B) (Done SOL altAB) ->
+    (exists altA, run s1 A (Done SOL altA)) \/ 
+      (exists altB, expand_no_cut_failure s1 A /\ run s2 B (Done SOL altB)).
 Proof.
   remember (Or _ _ _) as O1 eqn:HO1.
-  remember (Or A' _ _) as O2 eqn:HO2.
-  remember (Done _) as D eqn:HD.
+  remember (Done _ _) as D eqn:HD.
   move=> H.
-  elim: H s2 A A' B B' SOL HO1 HO2 HD; clear => //=.
-  + move=> s st s' + s2 A A' B B' SOL H; rewrite H => + [] ?? [] ?; subst => //=.
+  elim: H s2 A B altAB SOL HO1 HD; clear => //=.
+  + move=> s st s' alt + s2 A B altAB SOL ? []??; subst => //=.
     case E: expand => //=.
-      case F: expand => //= -[] ?; subst.
-      by right; repeat split; auto; [apply: expand_no_cut_failure_fail E| apply: run_done].
-    move=> [] ?; subst; left.
-    apply: run_done E.
-  + move=> s ? st1 st2 ? + H1 IH s2 A A' B B' SOL ???; subst => /=.
+    + case F: expand => //= -[] ??; subst.
+      right; eexists; repeat split.
+      + apply: expand_no_cut_failure_fail E.
+      + apply: run_done F.
+    + move=> [] ??; subst; left.
+      eexists; apply: run_done E.
+  + move=> s ? st1 st2 + H1 IH s2 A B altAB SOL ??; subst => /=.
     case E: expand => //=.
     by case F: expand => //=.
-  + move=> s ? st1 st2 ? + H1 IH s2 A A' B B' SOL ??? ; subst => //=.
+  + move=> s ? st1 st2 + H1 IH s2 A B altAB SOL ?? ; subst => //=.
     case E: expand => [s4|||s4] //=.
     + move=> [] ?; subst.
-      move: IH => /(_ _ _ _ _ _ _ erefl erefl erefl) [H|[HL HR]].
-      - left; apply: run_step E H.
-      - by right; split; [apply: expand_no_cut_failure_step E HL|assumption].
+      move: IH => /(_ _ _ _ _ _ erefl erefl) [[altA H]|[altA[HL HR]]].
+      - left; eexists; apply: run_step E H.
+      - right; eexists; split; [apply: expand_no_cut_failure_step E HL|apply: HR].
     + move=> [] ?; subst.
-      move: IH => /(_ _ _ _ _ _ _ erefl erefl erefl) [H|[HL HR]].
-      - by left; apply: run_cut E H.
-      - by right; split; auto; move: (run_cut_fail HR).
+      move: IH => /(_ _ _ _ _ _ erefl erefl) [[altA H]|[?[HL HR]]].
+      - by left; eexists; apply: run_cut E H.
+      - by move: (run_cut_fail HR).
     + case F: expand => [ss|ss||] //=.
       - move=> [] ?; subst.
-        move: IH => /(_ _ _ _ _ _ _ erefl erefl erefl) [H|[HL HR]].
+        move: IH => /(_ _ _ _ _ _ erefl erefl) [[? H]|[?[HL HR]]].
         by destruct (run_Failure_and_Done E H).
-        right; split; auto; apply: run_step F HR.
+        right; eexists; split; auto; apply: run_step F HR.
       - move=> [] ?; subst.
-        move: IH => /(_ _ _ _ _ _ _ erefl erefl erefl) [H|[HL HR]].
+        move: IH => /(_ _ _ _ _ _ erefl erefl) [[? H]|[? [HL HR]]].
         by destruct (run_Failure_and_Done E H).
-        by right; split; auto; apply: run_cut F HR.
+        right; eexists; split; auto; apply: run_cut F HR.
 Qed.
 
-Lemma run_expand_no_cut_failure {s A ign} : 
-  expand_no_cut_failure s A ign -> 
-    run s A Failed ign.
+Lemma run_expand_no_cut_failure {s A} : 
+  expand_no_cut_failure s A -> 
+    run s A Failed.
 Proof.
-  move=> H; elim: H => [{}s {}st| {}s {}st st1 st2] H.
+  move=> H; elim: H => [{}s {}st| {}s {}st st2] H.
   + by apply: run_fail H.
-  + by move=> _ H2; apply: run_step H H2.
+  + move=> H2; apply: run_step H.
 Qed.
 
-Lemma expand_no_cut_failure_expanded {s1 s2 g1 g2}:
+Lemma expand_no_cut_failure_expanded {s1 s2 g1}:
    expand s1 g1 = Expanded s2 ->
-    expand_no_cut_failure s1 g1 g2 ->
-      expand_no_cut_failure s1 s2 g2.
+    expand_no_cut_failure s1 g1 ->
+      expand_no_cut_failure s1 s2.
 Proof.
   move=> + H; elim: H s2; [congruence|]; clear.
-  move=> s1 st st1 g2 H; rewrite H => H1 IH g1 []?; subst.
+  move=> s1 st st1 H; rewrite H => H1 IH g1 []?; subst.
   inversion H1; clear H1; subst.
   - by apply: expand_no_cut_failure_fail.
   - by apply: expand_no_cut_failure_step (H0) _; apply IH.
 Qed.
 
-Lemma run_or_fail {s1 s2 g1 g2 st}:
-  run s1 (Or g1 s2 g2) Failed st ->
-    run s1 g1 Failed st /\ (expand_no_cut s1 g1 -> run s2 g2 Failed st).
+Lemma run_or_fail {s1 s2 g1 g2}:
+  run s1 (Or g1 s2 g2) Failed ->
+    run s1 g1 Failed /\ (expand_no_cut s1 g1 -> run s2 g2 Failed).
 Proof.
   move=> H.
   remember (Or _ _ _) as O eqn:HO.
   remember Failed as F eqn:HF.
   move: s2 g1 g2 HO HF.
   elim: H; clear => //=.
-  + move=> s st s' + s2 g1 g2 HO _; subst => /=.
+  + move=> s s' + s2 g1 g2 HO _; subst => /=.
     case E: expand => //=.
     case F: expand => //=.
     by move=> _; split; intros; apply run_fail.
-  + move=> s ? st1 st2 ? + H1 IH s2 g1 g2 ? ?; subst => /=.
+  + move=> s st1 st2 ? + H1 IH s2 g1 g2 ? ?; subst => /=.
     case E: expand => //=.
     by case F: expand => //=.
-  + move=> s ? st1 st2 ? + H1 IH s2 g1 g2 ?? ; subst => //=.
+  + move=> s st1 st2 ? + H1 IH s2 g1 g2 ?? ; subst => //=.
     case E: expand => [s4|||s4] //=.
     + move=> [] ?; subst.
       move: (IH _ _ _ erefl erefl) => [] HL HR {IH}.
@@ -633,36 +614,36 @@ Lemma expand_no_cut_cut {s A B}:
   expand_no_cut s A -> expand s A = CutBrothers B -> False.
 Proof. by move=> H; elim: H B; congruence. Qed.
 
-Lemma run_Failed_cut {s s2 A B X Y}:
-   run s A Failed X ->
-    run s (Or A s2 (cut B)) Failed Y.
+Lemma run_Failed_cut {s s2 A B}:
+   run s A Failed ->
+    run s (Or A s2 (cut B)) Failed.
 Proof.
   remember Failed as F eqn:HF.
   move=> H.
-  elim: H s2 B Y HF; clear => //=.
-  + move=> s A _ H s2 B Y _.
+  elim: H s2 B HF; clear => //=.
+  + move=> s A H s2 B _.
     move: (expand_cut_result1 s2 B) => [ | [D]] H1.
     + by apply: run_fail => //=; rewrite H H1.
     + by move: (expand_cut_expanded H1).
-  + move=> s A st1 st2 r H H1 IH s2 B Y ?; subst.
+  + move=> s s' st1 st2 H H1 IH s2 B ?; subst.
     apply: run_step => //=.
     + by rewrite H.
     + apply: IH erefl.
-  + move=> s A st1 st2 r H H1 IH s2 B Y ?; subst.
+  + move=> s s' st1 st2 H H1 IH s2 B ?; subst.
     apply: run_step => //=.
     + by rewrite H.
     + apply: IH erefl.
 Qed.
 
-Lemma run_or_fail1 {s1 s2 g1 g2 st aa}:
-    run s1 g1 Failed aa -> (expand_no_cut s1 g1 -> run s2 g2 Failed st) ->
-      run s1 (Or g1 s2 g2) Failed st.
+Lemma run_or_fail1 {s1 s2 g1 g2}:
+    run s1 g1 Failed -> (expand_no_cut s1 g1 -> run s2 g2 Failed) ->
+      run s1 (Or g1 s2 g2) Failed.
 Proof.
   move: (classic (expand_no_cut s1 g1)) => [].
   + move=> H + /(_ H) => H1; move: H.  
     remember Failed as F eqn:HF.
-    elim: H1 s2 g2 st HF; clear => //=.
-    + move=> s A _ H s2 B C _ H1 H2; subst.
+    elim: H1 s2 g2 HF; clear => //=.
+    + move=> s A H s2 B _ H1 H2; subst.
       remember Failed as F eqn:HF.
       elim: H2 s A H H1 HF; clear => //=.
       + by intros; apply run_fail => //=; rewrite H0 H1.
@@ -683,9 +664,9 @@ Proof.
   + remember Failed as F eqn:HF.
     remember (Or _ _) as O eqn:HO.
     move=> H1 H _.
-    elim: H H1 s2 g2 st HF O HO; clear => //=.
-    + by move=> s st st1 H []; apply expand_no_cut_failure1.
-    + move=> s st st1 st2 r H H1 IH H2 s2 g2 st0 ? O HO; subst.
+    elim: H H1 s2 g2 HF O HO; clear => //=.
+    + by move=> s st1 H []; apply expand_no_cut_failure1.
+    + move=> s st1 st2 r H H1 IH H2 s2 g2 ? O HO; subst.
       apply: run_step => //=.
       + rewrite H => //=.
       + apply: run_Failed_cut H1.
