code/rocq/aux.v
@@ -1,61 +1,27 @@
 From mathcomp Require Import all_ssreflect.
 From det Require Import det.
 
-Lemma run_consistent_res {a b c1 c2 r1 r2}:
-  run a b c1 r1 -> run a b c2 r2 -> c1 = c2.
-Proof. by move=> H H1; apply (proj1 (run_consistent H H1)). Qed.
+Lemma run_consistent_res {a b c1 c2}:
+  run a b c1 -> run a b c2 -> c1 = c2.
+Proof. by move=> H H1; apply ((run_consistent H H1)). Qed.
 
-Lemma run_consistent_state {a b c1 c2 r1 r2}:
-    run a b c1 r1 -> run a b c2 r2 -> (c1 <> Failed ->  r1 = r2).
-Proof. by move=> H H1; apply (proj2 (run_consistent H H1)). Qed.
-
-Lemma run_CutBrothers_id {s2 s3 st1 st2 ir1 ir2}:
-  expand s3 st1 = CutBrothers st2 -> 
-  run s3 st2 (Done s2) ir1 -> 
-  run s3 st1 (Done s2) ir2 ->
-  ir1 = ir2.
-Proof.
-  move: s2 s3 st2 ir1 ir2.
-  case: st1 => //=.
-  + move=> pr [] //=.
-    - move=> ????? [] <- H => //= H1.
-      apply run_cut_simpl in H1 as []; subst; by inversion H.
-    - move=> [] pn args s2 s3 st2 ir1 ir2 => //=; by case F: F => [|[]] //=.
-  + by move=> st0  s st1 s2 s3 st2 ir1 ir2; by case: expand; case: expand => //.
-  + move=> st0 st1 s2 s3 st2 ir1 ir2 + + H.
-    move: (run_and_complete H) => [il [ir [s'' [?[HL HR]]]]]; subst.
-    case E: expand => //; inversion HL; try congruence; subst.
-    + move: E; rewrite H0 => -[] ? [] ? H2; subst.
-      move: (run_and_complete H2) => [il2 [ir2 [s'''[?[HL' HR']]]]]; subst.
-      move: (run_consistent H1 HL') => [][] ? /(_ done_fail) ?; subst.
-      by move: (run_consistent HR HR') => [] _ /(_ done_fail) ?; subst.
-    + move: E; rewrite H3 => -[]?; subst.
-      case F: expand => //= -[] ? H1; subst.
-      move: (run_and_complete H1) => [il1 [ir2 [s''1 [?[HL1 HR1]]]]] {H1}; subst.
-      move: (run_consistent HL1 HL) => [][] ? /(_ done_fail) ?; subst.
-      inversion HR; try congruence; subst.
-      move: H0; rewrite F => -[] ?; subst.
-      by move: (run_consistent HR1 H1) => [] _ /(_ done_fail) ?; subst.
-Qed.
-
-
-Lemma expand_no_cut_split {s A B sol st}:
+Lemma expand_no_cut_split {s A B sol alts}:
   expand_no_cut s (And A B) ->
-    expand_no_cut s A /\ (run s A (Done sol) st -> expand_no_cut sol B).
+    expand_no_cut s A /\ (run s A (Done sol alts) -> expand_no_cut sol B).
 Proof.
   remember (And _ _) as NA eqn:HNA.
   move=> H.
-  move: A B sol st HNA.
+  move: A B sol HNA alts.
   elim: H; clear.
-  + move=> sol s ? H A B sol1 A' ?; subst.
+  + move=> sol s ? alt H A B sol1 ?; subst.
     move: H => //=.
     case E: expand => //=.
     case F: expand => //= -[] ?; subst.
     split.
       - by apply: expand_no_cut_solved E.
-      - move=> H1; move: (run_Solved_id E H1) => [][]??; subst.
+      - move=> H1; move: (run_Solved_id E H1) => []??; subst.
         apply: expand_no_cut_solved F.
-  + move=> s g + A B sol A' ?; subst => //=.
+  + move=> s g + A B sol ?; subst => //=.
     case E: expand => //=.
     - move=> _; split.
       by apply: expand_no_cut_failure1.
@@ -63,34 +29,34 @@ Proof.
     - case F: expand => //=.
       move=> _; split.
       by apply: expand_no_cut_solved E.
-      move=> H; move: (run_Solved_id E H) => [][]??; subst.
+      move=> H; move: (run_Solved_id E H) => []??; subst.
       by apply: expand_no_cut_failure1.
-  + move=> s g g' + H1 IH A B sol A' ?; subst => //=.
-    case E: expand => [|||sol'] //=.
-    - move=> [] ?; subst.
-      move: IH => /(_ _ _ sol A' erefl) [] H2 H3; split.
+  + move=> s g g' + H1 IH A B sol ?; subst => //=.
+    case E: expand => [|||sol' alts'] //=.
+    - move=> [] ? alts; subst.
+      move: IH => /(_ _ _ sol erefl alts) [] H2 H3; split.
       - by apply: expand_no_cut_expanded E H2.
       - by move=> H; apply H3; inversion H; subst; clear H; congruence.
     - case F: expand => [A''|||] //= -[] ?; subst.
       split.
       - by apply: expand_no_cut_solved E.
       - move=> H.
-        move: (run_Solved_id E H)=> [][]??; subst.
-        move: IH => /(_ _ _ sol' A' erefl) => -[] H2 H3. 
+        move: (run_Solved_id E H)=> []??; subst.
+        move: IH => /(_ _ _ sol' erefl alts') => -[] H2 H3. 
         by apply: expand_no_cut_expanded F (H3 H).
 Qed.
 
-Lemma expand_no_cut_failure_run {s A B}:
-  expand_no_cut_failure s A B -> run s A Failed B.
+Lemma expand_no_cut_failure_run {s A}:
+  expand_no_cut_failure s A -> run s A Failed.
 Proof.
   move=> H; elim: H; clear.
   + by constructor.
-  + by move=> s A st1 B H H1 H2; apply: run_step H H2.
+  + by move=> s A st1 H H1 H2; apply: run_step H H2.
 Qed.
 
-Corollary run_or_fail1 s1 g1 g2 st:
-  run s1 (Or g1 s1 g2) Failed st ->
-    run s1 g1 Failed st /\ (expand_no_cut s1 g1 -> run s1 g2 Failed st).
+Corollary run_or_fail1 s1 g1 g2:
+  run s1 (Or g1 s1 g2) Failed ->
+    run s1 g1 Failed /\ (expand_no_cut s1 g1 -> run s1 g2 Failed).
 Proof. move=> H. apply: run_or_fail H. Qed. 
 
 Lemma not_cut_borothers_expanded_and_left {s A B ss}:
@@ -102,14 +68,14 @@ Proof.
   move=> H.
   move: A B HAnd ss.
   case: H; clear => //=.
-  by move=> ??? + ???? H; subst => //=; rewrite H.
+  by move=> ???? + ???? H; subst => //=; rewrite H.
   by move=> ?? + ???? H; subst => //=; rewrite H.
   by move=> ??? + H1 ???? H2; subst => //=; rewrite H2 => -[] ?; subst; auto.
 Qed.
 
-Lemma not_cut_borothers_expanded_and_right {s A B B'' ss}:
+Lemma not_cut_borothers_expanded_and_right {s A B B'' ss altA}:
   expand_no_cut s (And A B) ->
-    expand s A = Solved ss ->
+    expand s A = Solved ss altA ->
     expand ss B = Expanded B'' ->
       expand_no_cut s (And A B'').
 Proof.
@@ -117,61 +83,58 @@ Proof.
   move=> H.
   move: A B HAnd ss B''.
   case: H; clear => //=.
-  by move=> ??? + ????? H H1; subst => //=; rewrite H H1.
+  by move=> ???? + ????? H H1; subst => //=; rewrite H H1.
   by move=> ?? + ????? H H1; subst => //=; rewrite H H1.
   by move=> ??? + H1 H2 ???? H3 H4; subst => //=; rewrite H3 H4 => -[] ?; subst; auto.
 Qed.
 
-Lemma p_aorb_andc {sA sB sD A B C D E}:
-  run sA (And (Or A sB B) C) (Done sD) D ->
-    run sA (And A C) Failed E ->
-      exists D', run sB (And B C) (Done sD) D'.
+Lemma p_aorb_andc {sA sB sD A B C alts}:
+  run sA (And (Or A sB B) C) (Done sD alts) ->
+    run sA (And A C) Failed ->
+      exists alts, run sB (And B C) (Done sD alts).
 Proof.
   move=> H H1.
-  move: (run_and_complete H) => [il[ir[s'' [?[HAORB HC]]]]] {H}; subst.
-  move: (run_or_done HAORB) => [A' [B' ?]]; subst.
+  move: (run_and_complete H) => [s'' [altL [altR [? [HAORB HC]]]]] {H}; subst.
   move: (run_or_complete HAORB) => [].
-    + move=> HA; move: (run_and_fail H1) => [HA'|].
-      + move: (run_consistent HA HA') => []; by [].
-      + move=> [X[Y [HA' HC']]].
-        move: (run_consistent HA HA') => [] [] ? /(_ done_fail) ?; subst.
-        by move: (run_consistent HC HC') => [].
-    + move=> [] HA HB.
-      exists (And B' ir).
-      apply: run_and_correct HB HC.
+    + move=> [altA HA]; move: (run_and_fail H1) => [].
+      + move=> HA'; move: (run_consistent HA HA'); by [].
+      + move=> [X [altA0 [HA' HC']]].
+        move: (run_consistent HA HA') => [] ?; subst.
+        by move: (run_consistent HC HC').
+    + move=> [] alts [] HA HB.
+      eexists; apply: run_and_correct HB HC.
 Qed.
 
 (* ((A ∧ B) ∨ (A ∧ C)) -> (A ∧ (B ∨ C)) *)
-Lemma or_is_distributive {A B C s sol E}:
-    run s (Or (And A B) s (And A C)) (Done sol) E ->
+Lemma or_is_distributive {A B C s sol alts}:
+    run s (Or (And A B) s (And A C)) (Done sol alts) ->
       expand_no_cut s (And A B) ->
-        exists E' s' IGN, run s A (Done s') IGN /\
-          run s (And A (Or B s' C)) (Done sol) E' .
+        exists s' altA altABC, run s A (Done s' altA) /\
+          run s (And A (Or B s' C)) (Done sol altABC) .
 Proof.
   move=> H H1.
-  move: (run_or_done H) => [AB [AC ?]]; subst.
   move: (run_or_complete H) => [].
   (* left succeeds *)
-  + move=> HAB. move: (run_and_done HAB) => [A' [B' ?]]; subst.
-    move: (run_and_complete HAB) => [il[ir[s'' [+ [HA HB]]]]] {H} => -[]??; subst.
-    move: (run_or_correct_left HB s'' C) => [] X H.
-    do 3 eexists; split; [apply: HA|].
+  + move=> [altAB HAB].
+    move: (run_and_complete HAB) => [s'' [? [? [? [HA HB]]]]] {H}; subst.
+    move: (run_or_correct_left HB s'' C) => [altB H].
+    repeat eexists; [apply: HA|].
     apply: run_and_correct (HA) H.
   (* right succeeds *)
-  + move=> [] EAB HAC; move: (run_and_complete HAC) => [il[ir[s'' [?[HA HC]]]]] {HAC}; subst.
+  + move=> [] altB [] EAB HAC; move: (run_and_complete HAC) => [s'' [?[?[?[HA HC]]]]] {HAC}; subst.
     move: (run_and_fail (run_expand_no_cut_failure EAB)) => [H0|].
-    + by move: (run_consistent H0 HA) => [].
-    + move=> [s1 [s2 [HA' HB]]].
-      move: (run_consistent HA HA') => [] [] ? /(_ done_fail) ?; subst.
+    + by move: (run_consistent H0 HA).
+    + move=> [s1 [altA [HA' HB]]].
+      move: (run_consistent HA HA') => [] ??; subst.
       move: (expand_no_cut_failure_split EAB) => [].
-      + by move=> []? H2; move: (run_consistent (run_expand_no_cut_failure H2) HA') => [].
-        move=> [s' [A' [B' [H2 H3]]]].
+      + by move=> H2; move: (run_consistent (run_expand_no_cut_failure H2) HA').
+      + move=> [s' [altA0 [H2 H3]]].
         (* move: (run_expand_all_solved H2 HA') => ?; subst. *)
-        move: (run_or_correct_right H3 HC) => [] p {}H.
-        move: (run_consistent HA H2) => [][]? /(_ done_fail) ?; subst.
-        do 3 eexists; split.
+        move: (run_or_correct_right H3 HC) => {}H.
+        move: (run_consistent HA H2) => []?; subst.
+        repeat eexists.
         + apply HA.
-        + apply: run_and_correct HA H.
+        + apply: run_and_correct H2 H.
 Qed.
 
 Lemma expand_cut_result {s A r}:
@@ -192,24 +155,4 @@ Proof.
     + by left; eexists.
     + apply IH1 in H as [[]|?] => //=.
     + apply IH1 in H as [[]|?] => //=.
-Qed.
-
-Lemma run_or_done_cut1 {s1 s2 SOL A A' B B'}:
-  run s1 (Or A s2 (cut B)) (Done SOL) (Or A' s2 B') -> B' = (cut B).
-Proof.
-  remember (Or A _ _) as O1 eqn:HO1.
-  remember (Or A' _ _) as O2 eqn:HO2.
-  remember (Done _) as D eqn:HD.
-  move=> H.
-  elim: H s2 A A' B B' SOL HO1 HO2 HD; clear => //=.
-  + by move=> s st s' H s2 A A' B B' SOL H1; rewrite H1 => -[] ?? [] ?; subst.
-  + move=> s st st1 st2 r + H1 IH s2 A A' B B' SOL ???; subst => //=.
-    by case E: expand => //=; case: expand => //=.
-  + move=> s st s1 st2 r + H1 IH s2 A A' B B' SOL ???; subst => //=.
-    case E: expand => //=.
-    + by move=> []?; subst; apply: IH erefl erefl erefl.
-    + by move=> []?; subst; apply: IH erefl erefl; rewrite cut_cut_same.
-    + case F: expand => //=.
-      + by move: (expand_cut_expanded F).
-      + by move: (expand_cut_CB F).
 Qed.
